More work on Pthread-style (dry) concurrency semantics

linking/compcert_threads.v
@@ -11,7 +11,7 @@ Set Implicit Arguments.
 
 (*NOTE: because of redefinition of [val], these imports must appear 
   after Ssreflect eqtype.*)
-Require Import AST.    (*for typ*)
+Require Import AST.     (*for typ*)
 Require Import Values. (*for val*)
 Require Import Globalenvs. 
 Require Import Memory.
@@ -19,9 +19,63 @@ Require Import Integers.
 
 Require Import ZArith.
 
+Notation EXIT := 
+  (EF_external 1%positive (mksignature (AST.Tint::nil) None)). 
+Notation FORK := 
+  (EF_external 2%positive 
+  (mksignature (AST.Tint::AST.Tint::nil) (Some AST.Tint))).
+Notation READ := 
+  (EF_external 3%positive 
+  (mksignature (AST.Tint::AST.Tint::AST.Tint::nil) (Some AST.Tint))).
+Notation WRITE := 
+  (EF_external 4%positive 
+  (mksignature (AST.Tint::AST.Tint::AST.Tint::nil) (Some AST.Tint))).
+Notation MKLOCK := 
+  (EF_external 5%positive (mksignature (AST.Tint::nil) (Some AST.Tint))).
+Notation FREE_LOCK := 
+  (EF_external 6%positive (mksignature (AST.Tint::nil) (Some AST.Tint))).
+Notation LOCK_SIG := (mksignature (AST.Tint::nil) (Some AST.Tint)).
+Notation LOCK := (EF_external 7%positive LOCK_SIG).
+Notation UNLOCK_SIG := (mksignature (AST.Tint::nil) (Some AST.Tint)).
+Notation UNLOCK := (EF_external 8%positive UNLOCK_SIG).
+
 Require Import compcert_linking.
 
-(** ** [ThreadPool.t] *)
+Definition access_map := Maps.PMap.t (Z -> perm_kind -> option permission).
+
+Module PermMap. Section PermMap.
+
+Record t := mk
+  { next : block
+  ;  map : access_map 
+  ;  max : forall (b : positive) (ofs : Z),
+                 Mem.perm_order'' (Maps.PMap.get b map ofs Max)
+                 (Maps.PMap.get b map ofs Cur)
+  ; nextblock : forall (b : positive) (ofs : Z) (k : perm_kind),
+                       ~ Coqlib.Plt b next -> Maps.PMap.get b map ofs k = None
+  }. 
+
+End PermMap. End PermMap.
+
+Section permMapDefs.
+
+Definition updPermMap (m : mem) (p : PermMap.t) : option mem :=
+  match positive_eq_dec (Mem.nextblock m) (PermMap.next p) with
+    | left pf => 
+        Some (Mem.mkmem 
+                        (Mem.mem_contents m) 
+                        (PermMap.map p) 
+                        (Mem.nextblock m)
+                        (PermMap.max p) 
+                        (eq_rect_r 
+                           (fun n => forall (b : positive) (ofs : Z) (k : perm_kind),
+                             ~ Coqlib.Plt b n -> Maps.PMap.get b (PermMap.map p) ofs k = None)
+                           (PermMap.nextblock p) pf)
+                        (Mem.contents_default m))
+    | right _ => None
+  end.
+
+End permMapDefs.
 
 Module ThreadPool. Section ThreadPool.
 
@@ -30,753 +84,136 @@ Variable sem : Modsem.t.
 Notation cT := (Modsem.C sem).
 
 Inductive ctl : Type :=
-| Krun : cT -> ctl
-| Klock : block -> Z -> cT -> ctl.
+  | Krun : cT -> ctl
+  | Klock : block -> Z -> cT -> ctl.
 
 Record t := mk
   { num_threads : pos
-  ; pool  :> 'I_num_threads -> cT
+  ; pool         :> 'I_num_threads -> ctl
+  ; counter   : nat
   }.
 
 End ThreadPool. End ThreadPool.
+
+Arguments ThreadPool.Krun [sem] _.
+Arguments ThreadPool.Klock [sem] _ _ _.
 
 Notation pool := ThreadPool.t.
 
 Section poolDefs.
 
-Context {sem : Modsem.t} (tp : pool sem).
+Context {sem : Modsem.t} {next : block}.
+
+Variable (tp : ThreadPool.t sem).
 
 Import ThreadPool.
 
 Notation cT := (Modsem.C sem).
-
-Definition addThread (c : cT) := 
-  let: new_num_threads := pos_incr (num_threads tp) in
-  let: new_tid := ordinal_pos_incr (num_threads tp) in
-  @mk sem new_num_threads  
-  (fun (n : 'I_new_num_threads) => 
-     if n == new_tid then c else tp n).
-
-Definition updStack (newStack : CallStack.t my_cores) :=
-  {| fn_tbl := l.(fn_tbl)
-   ; stack  := newStack |}.
-
-(** [inContext]: The top core on the call stack has a return context  *)     
-
-Definition inContext (l0 : linker N my_cores) := callStackSize l0.(stack) > 1.
-
-(** [updCore]: Replace the top core on the call stack with [newCore]  *)     
-
-Program Definition updCore (newCore: Core.t my_cores) := 
-  updStack (CallStack.mk (STACK.push (STACK.pop l.(stack)) newCore) _).  
-Next Obligation. apply/andP; split=>/=; last by []; by apply: callStack_ext. Qed.
-
-Lemma updCore_inj newCore newCore' : 
-  updCore newCore = updCore newCore' -> newCore=newCore'.
-Proof. by case. Qed.
-
-Lemma updCore_inj_upd c c1 c2 : 
-  updCore (Core.upd c c1) = updCore (Core.upd c c2) -> c1=c2.
-Proof. 
-case=> H1; move: (EqdepFacts.eq_sigT_snd H1); move=> <-.
-by rewrite -Eqdep.Eq_rect_eq.eq_rect_eq.
-Qed.
-
-(** [pushCore]: Push a new core onto the call stack.                       *)
-(** Succeeds only if all cores are currently at_external.                  *)
-
-Lemma stack_push_wf newCore :
-  all (atExternal my_cores) l.(stack).(callStack) -> 
-  wf_callStack (SeqStack.updStack (newCore :: l.(stack).(callStack))).
-Proof.
-by rewrite/wf_callStack=> H; apply/andP; split.
-Qed.
-
-Definition pushCore 
-  (newCore: Core.t my_cores) 
-  (pf : all (atExternal my_cores) l.(stack).(callStack)) := 
-  updStack (CallStack.mk (STACK.push l.(stack) newCore) (stack_push_wf _ pf)).
-
-(** [popCore]: Pop the top core on the call stack.                         *)
-(** Succeeds only if the top core is running in a return context.          *)
-
-Lemma inContext_wf (stk : Stack.t (Core.t my_cores)) : 
-  size stk > 1 -> wf_callStack stk -> wf_callStack (STACK.pop stk).
-Proof.
-rewrite/wf_callStack=> H1; move/andP=> [H2 H3]; apply/andP; split.
-- by apply: STACK.all_pop.
-- by move: H1 H2 H3; case: stk.
-Qed.
-
-Program Definition popCore : option (linker N my_cores) := 
-  (match inContext l as pf 
-         return (pf = inContext l -> option (linker N my_cores)) with
-    | true => fun pf => 
-        Some (updStack (CallStack.mk (STACK.pop l.(stack)) 
-                                     (inContext_wf _ _ _)))
-    | false => fun pf => None
-  end) Logic.eq_refl.
-Next Obligation. by apply: callStack_wf. Qed.
-
-Definition peekCore := STACK.head l.(stack) (callStack_nonempty l.(stack)).
-
-Definition emptyStack := if l.(stack).(callStack) is [::] then true else false.
-
-Import Modsem.
-
-(* We take the RC initial core here because we want to make sure the args *)
-(* are properly stashed in the [c] tuple.                                 *)
-
-Definition initCore (sg: signature) (ix: 'I_N) (v: val) (args: list val) 
-  : option (Core.t my_cores):=
-  if @initial_core _ _ _ 
-       (my_cores ix).(sem)
-       (my_cores ix).(Modsem.ge) 
-       v args 
-  is Some c then Some (Core.mk _ my_cores ix c sg)
-  else None.
-
-End linkerDefs.
-
-Notation ge_ty := (Genv.t unit unit).
-
-Arguments updStack {N} {my_cores} !_ _ /.
-
-Arguments updCore {N} {my_cores} !_ _ /.
-
-Arguments pushCore {N} {my_cores} !l _ _ /.
-
-Arguments peekCore {N} {my_cores} !l /.
-
-Arguments emptyStack {N} {my_cores} !l /.
-
-Lemma popCoreI N my_cores l l' pf : 
-  inContext l -> 
-  l' = updStack l (CallStack.mk (STACK.pop (CallStack.callStack l)) pf) ->
-  @popCore N my_cores l = Some l'.
-Proof.
-rewrite /popCore.
-move: (popCore_obligation_1 l); move: (popCore_obligation_2 l).
-case: (inContext l)=> pf1 pf2 // _ ->.
-f_equal=> //.
-f_equal=> //.
-f_equal=> //.
-by apply: proof_irr.
-Qed.
-
-Lemma popCoreE N my_cores l l' : 
-  @popCore N my_cores l = Some l' ->
-  exists pf,
-  [/\ inContext l
-    & l' = updStack l (CallStack.mk (STACK.pop (CallStack.callStack l)) pf)].
-Proof.
-rewrite /popCore.
-move: (popCore_obligation_1 l); move: (popCore_obligation_2 l).
-case: (inContext l)=> pf1 pf2 //; case=> <-.
-have pf: wf_callStack (STACK.pop (CallStack.callStack l)).
-{ case: (andP (pf1 erefl))=> A B; apply/andP; split=> //.
-  by apply: SeqStack.all_pop.
-  by move: (pf2 erefl); clear pf1 pf2 A B; case: l=> /= ?; case; elim. }
-exists pf; split=> //.
-by f_equal; f_equal; apply: proof_irr.
-Qed.
-
-(** **                     Linking Interaction Semantics                  *)
-
-Module LinkerSem. Section linkerSem.
-
-Variable N : pos.  (* Number of translation units *)
-Variable my_cores : 'I_N  -> Modsem.t.
-Variable my_fn_tbl: ident -> option 'I_N.
-
-(* [handle id l args] looks up function id [id] in function table         *)
-(* [l.fn_tbl], producing an optional module index [ix : 'I_N].  The index *)
-(* is used to construct a new core to handle the call to function         *)
-(* [id]. The new core is pushed onto the call stack.                      *)
-
-Section handle.
-
-Variables (sg: signature) (id: ident) (l: linker N my_cores) (args: list val).
-
-Import CallStack.
-
-Definition handle :=
-  (match all (atExternal my_cores) l.(stack).(callStack) as pf 
-        return (all (atExternal my_cores) l.(stack).(callStack) = pf
-               -> option (linker N my_cores)) with
-    | true => fun pf => 
-        if l.(fn_tbl) id is Some ix then
-        if Genv.find_symbol (my_cores ix).(Modsem.ge) id is Some bf then
-        if initCore my_cores sg ix (Vptr bf Int.zero) args is Some c 
-          then Some (pushCore l c pf)
-        else None else None else None
-    | false => fun _ => None
-  end) erefl.
-
-End handle.
-
-Section handle_lems.
-
-Import CallStack.
-
-Lemma handleP sg id l args l' :
-  handle sg id l args = Some l' <-> 
-  (exists (pf : all (atExternal my_cores) l.(stack).(callStack)) ix bf c,
-     [/\ l.(fn_tbl) id = Some ix 
-       , Genv.find_symbol (my_cores ix).(Modsem.ge) id = Some bf
-       , initCore my_cores sg ix (Vptr bf Int.zero) args = Some c
-       & l' = pushCore l c pf]).
-Proof.
-rewrite/handle.
-rewrite /pushCore.
-generalize (stack_push_wf l).
-pattern (all (atExternal my_cores) (CallStack.callStack (stack l))) 
- at 1 2 3 4 5 6 7 8.
-case f: (all _ _); move=> pf.
-case g: (fn_tbl l id)=> [ix|].
-case fnd: (Genv.find_symbol _ _)=> [bf|].
-case h: (initCore _ _ _)=> [c|].
-split=> H.
-exists (erefl true),ix,bf,c; split=> //; first by case: H=> <-.
-case: H=> pf0 []ix0 []bf0 []c0 []; case=> <-.
-rewrite fnd; case=> <-; rewrite h; case=> <- ->. 
-by repeat f_equal; apply: proof_irr.
-split=> //; case=> pf0 []ix0 []bf0 []c0 []. 
-by case=> <-; rewrite fnd; case=> <-; rewrite h.
-split=> //; case=> pf0 []ix0 []bf0 []c0 [].
-by case=> <-; rewrite fnd; discriminate.
-split=> //.
-by case=> pf0 []ix0 []bf0 []c0 []; discriminate.
-split=> //.
-by case=> pf0 []ix0 []bf0 []c0 []; discriminate.
-Qed.
-
-End handle_lems.
-
-Definition main_sig := mksignature nil (Some Tint).
-
-Definition initial_core (ge: ge_ty) (v: val) (args: list val)
-  : option (linker N my_cores) :=
-  if v is Vptr bf ofs then 
-  if Int.eq ofs Int.zero then
-  if Genv.invert_symbol ge bf is Some id then
-  if my_fn_tbl id is Some ix then
-  if initCore my_cores main_sig ix (Vptr bf Int.zero) args is Some c 
-  then Some (mkLinker my_fn_tbl (CallStack.singl c))
-  else None else None else None else None else None.
-
-(* Functions suffixed w/ 0 always operate on the running core on the (top *)
-(* of the) call stack.                                                    *)
-
-Definition at_external0 (l: linker N my_cores) :=
-  let: c   := peekCore l in
-  let: ix  := c.(Core.i) in                                            
-  let: sem := (my_cores ix).(Modsem.sem) in                        
-  let: F   := (my_cores ix).(Modsem.F) in                              
-  let: V   := (my_cores ix).(Modsem.V) in                              
-    @at_external (Genv.t F V) _ _ sem (Core.c c).
-
-Arguments at_external0 !l.
-
-Require Import val_casted. (*for val_has_type_func*)
-
-Definition halted0 (l: linker N my_cores) :=
-  let: c   := peekCore l in
-  let: ix  := c.(Core.i) in
-  let: sg  := c.(Core.sg) in
-  let: sem := (my_cores ix).(Modsem.sem) in
-  let: F   := (my_cores ix).(Modsem.F) in
-  let: V   := (my_cores ix).(Modsem.V) in
-  if @halted (Genv.t F V) _ _ sem (Core.c c) is Some v then
-    if val_casted.val_has_type_func v (proj_sig_res sg) then Some v
-    else None 
-  else None.
-
-Arguments halted0 !l.
-
-(* [corestep0] lifts a corestep of the runing core to a corestep of the   *)
-(* whole program semantics.                                               *)
-(* Note: we call the RC version of corestep here.                         *) 
-
-Definition corestep0 
-  (l: linker N my_cores) (m: Mem.mem) (l': linker N my_cores) (m': Mem.mem) := 
-  let: c   := peekCore l in
-  let: ix  := c.(Core.i) in
-  let: sem := (my_cores ix).(Modsem.sem) in
-  let: F   := (my_cores ix).(Modsem.F) in
-  let: V   := (my_cores ix).(Modsem.V) in
-  let: ge  := (my_cores ix).(Modsem.ge) in
-    exists c', 
-      @corestep (Genv.t F V) _ _ sem ge (Core.c c) m c' m'
-   /\ l' = updCore l (Core.upd c c').
-
-Arguments corestep0 !l m l' m'.
-
-Definition fun_id (ef: external_function) : option ident :=
-  if ef is (EF_external id sig) then Some id else None.
-
-(* The linker is [at_external] whenever the top core is [at_external] and *)
-(* the [id] of the called external function isn't handleable by any       *)
-(* compilation unit.                                                      *)
-
-Definition at_external (l: linker N my_cores) :=
-  if at_external0 l is Some (ef, dep_sig, args) 
-    then if fun_id ef is Some id then
-         if fn_tbl l id is None then Some (ef, dep_sig, args) else None
-         else None
-  else at_external0 l.
-
-(* We call the RC version of after_external here to ensure that the       *)
-(* return value [mv] of the external call is properly stashed in the      *)
-(* state tuple [c].                                                       *)
-
-Definition after_external (mv: option val) (l: linker N my_cores) :=
-  let: c   := peekCore l in
-  let: ix  := c.(Core.i) in
-  let: sem := (my_cores ix).(Modsem.sem) in
-  let: F   := (my_cores ix).(Modsem.F) in
-  let: V   := (my_cores ix).(Modsem.V) in
-  let: ge  := (my_cores ix).(Modsem.ge) in
-    if @after_external (Genv.t F V) _ _ sem mv (Core.c c) 
-      is Some c' then Some (updCore l (Core.upd c c'))
-    else None.
-
-(** The linker is [halted] when the last core on the call stack is halted. *)
-
-Definition halted (l: linker N my_cores) := 
-  if ~~inContext l then 
-  if halted0 l is Some rv then Some rv
-  else None else None.
-
-(** Return type of topmost core *)
-
-Definition retType0 (l: linker N my_cores) : option typ :=
-  let: c  := peekCore l in 
-  let: sg := c.(Core.sg) in 
-    sig_res sg.
-
-(** ** Corestep relation of linking semantics *)
-
-Definition corestep 
-  (l: linker N my_cores) (m: Mem.mem)
-  (l': linker N my_cores) (m': Mem.mem) := 
-
-  (** 1- The running core takes a step, or *)
-  corestep0 l m l' m' \/
-
-  (** 2- We're in a function call context. In this case, the running core is either *)
-  (m=m' 
-   /\ ~corestep0 l m l' m' 
-   /\
-      (** 3- at_external, in which case we push a core onto the stack to handle 
-         the external function call (or this is not possible because no module 
-         handles the external function id, in which case the entire linker is 
-         at_external) *)
-
-      if at_external0 l is Some (ef, dep_sig, args) then
-      if fun_id ef is Some id then
-      if handle (ef_sig ef) id l args is Some l'' then l'=l'' else False else False
-      else 
-
-      (** 4- or halted, in which case we pop the halted core from the call stack
-         and inject its return value into the caller's corestate. *)
-
-      if inContext l then 
-      if halted0 l is Some rv then
-      if popCore l is Some l0 then 
-      if after_external (Some rv) l0 is Some l'' then l'=l'' 
-      else False else False else False
-
-     else False).
-
-(** An inductive characterization of [corestep] above, proved equivalent below. *)
-
-Inductive Corestep : linker N my_cores -> mem 
-                     -> linker N my_cores -> mem -> Prop :=
-| Corestep_step : 
-  forall l m c' m',
-  let: c     := peekCore l in
-  let: c_ix  := Core.i c in
-  let: c_ge  := Modsem.ge (my_cores c_ix) in
-  let: c_sem := Modsem.sem (my_cores c_ix) in
-    semantics.corestep c_sem c_ge (Core.c c) m c' m' -> 
-    Corestep l m (updCore l (Core.upd (peekCore l) c')) m'
-
-| Corestep_call :
-  forall (l : linker N my_cores) m ef dep_sig args id bf d_ix d
-         (pf : all (atExternal my_cores) (CallStack.callStack l)),
-
-  let: c := peekCore l in
-  let: c_ix  := Core.i c in
-  let: c_ge  := Modsem.ge (my_cores c_ix) in
-  let: c_sem := Modsem.sem (my_cores c_ix) in
-
-  semantics.at_external c_sem (Core.c c) = Some (ef,dep_sig,args) -> 
-  fun_id ef = Some id -> 
-  fn_tbl l id = Some d_ix -> 
-  Genv.find_symbol (my_cores d_ix).(Modsem.ge) id = Some bf -> 
-
-  let: d_ge  := Modsem.ge (my_cores d_ix) in
-  let: d_sem := Modsem.sem (my_cores d_ix) in
-
-  semantics.initial_core d_sem d_ge (Vptr bf Int.zero) args = Some d -> 
-  Corestep l m (pushCore l (Core.mk _ _ _ d (ef_sig ef)) pf) m
-
-| Corestep_return : 
-  forall (l : linker N my_cores) l'' m rv d',
-
-  1 < CallStack.callStackSize (stack l) -> 
-
-  let: c  := peekCore l in
-  let: c_ix  := Core.i c in
-  let: c_sg  := Core.sg c in
-  let: c_ge  := Modsem.ge (my_cores c_ix) in
-  let: c_sem := Modsem.sem (my_cores c_ix) in
-
-  popCore l = Some l'' -> 
-
-  let: d  := peekCore l'' in     
-  let: d_ix  := Core.i d in
-  let: d_ge  := Modsem.ge (my_cores d_ix) in
-  let: d_sem := Modsem.sem (my_cores d_ix) in
-
-  semantics.halted c_sem (Core.c c) = Some rv -> 
-  val_has_type_func rv (proj_sig_res c_sg)=true -> 
-  semantics.after_external d_sem (Some rv) (Core.c d) = Some d' -> 
-  Corestep l m (updCore l'' (Core.upd d d')) m.
-
-Lemma CorestepE l m l' m' : 
-  Corestep l m l' m' -> 
-  corestep l m l' m'.
-Proof.
-inversion 1; subst; rename H0 into A; rename H into B.
-by left; exists c'; split.
-right; split=> //.
-split=> //.
-rewrite /corestep0=> [][]c' []step.
-by rewrite (corestep_not_at_external _ _ _ _ _ _ step) in A.
-rewrite /inContext /at_external0 A H1.
-case e: (handle _ _ _)=> //[l'|].
-move: e; case/handleP=> pf' []ix' []bf' []c []C G D ->.
-move: D; rewrite /initCore.
-rewrite H2 in C; case: C=> eq; subst ix'.
-rewrite G in H3; case: H3=> ->.
-by rewrite H4; case=> <-; f_equal; apply: proof_irr.
-move: e; rewrite/handle /pushCore.
-generalize (stack_push_wf l).
-pattern (all (atExternal my_cores) (CallStack.callStack (stack l))) 
- at 1 2 3 4 5 6.
-case f: (all _ _)=> pf'.
-rewrite H2 H3 /initCore H4; discriminate.
-by rewrite pf in f.
-right; split=> //.
-split=> //.
-rewrite /corestep0=> [][]c' []step.
-by rewrite (corestep_not_halted _ _ _ _ _ _ step) in H2.
-have at_ext: 
-  semantics.at_external
-    (Modsem.sem (my_cores (Core.i (peekCore l))))
-    (Core.c (peekCore l)) = None.
-{ case: (at_external_halted_excl 
-         (Modsem.sem (my_cores (Core.i (peekCore l))))
-         (Core.c (peekCore l)))=> //.
-  by rewrite H2. }
-rewrite /inContext A /at_external0 H1 at_ext.
-by rewrite /halted0 H2 /after_external H3 H4. 
-Qed.
-
-Lemma CorestepI l m l' m' : 
-  corestep l m l' m' -> 
-  Corestep l m l' m'.
-Proof.
-case.
-case=> c []step ->.
-by apply: Corestep_step.
-case=> <-.
-case=> nstep.
-case atext: (at_external0 _)=> [[[ef dep_sig] args]|//].
-case funid: (fun_id ef)=> [id|//].
-case hdl:   (handle (ef_sig ef) id l args)=> [l''|//] ->.
-move: hdl; case/handleP=> pf []ix []bf []c []fntbl genv init ->.
-move: init; rewrite /initCore.
-case init: (semantics.initial_core _ _ _ _)=> [c'|//]; case=> <-. 
-by apply: (@Corestep_call _ _ ef dep_sig args id bf).
-case inCtx: (inContext _)=> //.
-case hlt: (halted0 _)=> [rv|//].
-case pop: (popCore _)=> [c|//].
-case aft: (after_external _ _)=> [l''|//] ->.
-move: aft; rewrite /after_external.
-case aft: (semantics.after_external _ _ _)=> [c''|//]. 
-rewrite /halted0 in hlt; move: hlt.
-case hlt: (semantics.halted _ _)=> //. 
-case oval: (val_has_type_func _ _)=> //; case=> Heq. subst. case=> <-.
-by apply: (@Corestep_return _ _ _ rv c'').
-Qed.
-
-(** Prove that the two representations above coincide. *)
-
-Lemma CorestepP l m l' m' : 
-  corestep l m l' m' <-> Corestep l m l' m'.
-Proof. by split; [apply: CorestepI | apply: CorestepE]. Qed.
-
-Lemma corestep_not_at_external0 m c m' c' :
-  corestep0 c m c' m' -> at_external0 c = None.
-Proof. by move=>[]newCore []H1 H2; apply corestep_not_at_external in H1. Qed.
-
-Lemma at_external_halted_excl0 c : at_external0 c = None \/ halted0 c = None.
-Proof. 
-case: (at_external_halted_excl (Modsem.sem (my_cores (Core.i (peekCore c))))
-        (Core.c (peekCore c))).
-by rewrite /at_external0=> ->; left.
-by rewrite /halted0=> ->; right.
-Qed.
-
-Lemma corestep_not_halted0 m c m' c' : corestep0 c m c' m' -> halted c = None.
-Proof.
-move=> []newCore []H1 H2; rewrite/halted.
-case Hcx: (~~ inContext _)=>//; case Hht: (halted0 _)=>//.
-move: Hht; rewrite/halted0; apply corestep_not_halted in H1. 
-by move: H1=> /= ->. 
-Qed.
-
-Lemma corestep_not_halted0' m c m' c' : corestep0 c m c' m' -> halted0 c = None.
-Proof.
-move=> []newCore []H1 H2; rewrite/halted.
-case Hht: (halted0 _)=>//.
-by move: Hht; rewrite/halted0; apply corestep_not_halted in H1; rewrite /= H1.
-Qed.
-
-Lemma corestep_not_at_external (ge : ge_ty) m c m' c' : 
-  corestep c m c' m' -> at_external c = None.
-Proof.
-rewrite/corestep/at_external.
-move=> [H|[_ [_ H]]]; first by move: H; move/corestep_not_at_external0=> /= ->.
-move: H; case Heq: (at_external0 c)=>[[[ef sig] args]|//].
-move: Heq; case: (at_external_halted_excl0 c)=> [H|H]; first by rewrite H.
-move=> H2; case: (fun_id ef)=>// id; case hdl: (handle _ _ _)=> [a|].
-by move: hdl; case/handleP=> ? []? []? []? []->.
-by [].
-Qed.
-
-Lemma at_external0_not_halted c x :
-  at_external0 c = Some x -> halted c = None.
-Proof.
-case: (at_external_halted_excl0 c); rewrite/at_external0/halted.
-by case Heq: (peekCore c)=>//[a] ->.
-move=> H; case Heq: (peekCore c)=>//[a]. 
-by case Hcx: (~~ inContext _)=>//; rewrite H.
-Qed.
-
-Lemma corestep_not_halted (ge : ge_ty) m c m' c' :
-  corestep c m c' m' -> halted c = None.
-Proof. 
-rewrite/corestep.
-move=> [H|[_ [_ H]]]; first by move: H; move/corestep_not_halted0.
-move: H; case Hat: (at_external0 _)=> [x|//].
-by rewrite (at_external0_not_halted _ Hat).
-by rewrite /halted; case Hcx: (inContext _).
-Qed.
-
-Lemma at_external_halted_excl c :
-  at_external c = None \/ halted c = None.
-Proof.
-rewrite/at_external/halted; case Hat: (at_external0 c)=>//; 
-first by right; apply: (at_external0_not_halted _ Hat). 
-by left.
-Qed.
-
-Notation cast'' pf x := (cast (Modsem.C \o my_cores) (sym_eq pf) x).
-
-Lemma after_externalE rv c c' : 
-  after_external rv c = Some c' -> 
-  exists fn_tbl hd hd' tl pf pf' 
-         (eq_pf : Core.i hd = Core.i hd') 
-         (sig_pf : Core.sg hd = Core.sg hd'),
-  [/\ c  = mkLinker fn_tbl (CallStack.mk [:: hd & tl] pf)
-    , c' = mkLinker fn_tbl (CallStack.mk [:: hd' & tl]  pf')
-    & semantics.after_external
-       (Modsem.sem (my_cores (Core.i hd))) rv (Core.c hd)
-      = Some (cast'' eq_pf (Core.c hd'))].
-Proof.
-case: c=> fntbl; case; case=> // hd stk pf aft; exists fntbl,hd.
-move: aft; rewrite /after_external /=.
-case e: (semantics.after_external _ _ _)=> // [hd']; case=> <-.
-exists (Core.mk N my_cores (Core.i hd) hd' (Core.sg hd)),stk,pf,pf.
-rewrite /=; exists refl_equal; exists refl_equal; split=> //; f_equal; f_equal.
-by apply: proof_irr.
-Qed.
-
-(** Construct the interaction semantics of linking. *)
-
-Definition coresem : CoreSemantics ge_ty (linker N my_cores) Mem.mem :=
-  Build_CoreSemantics ge_ty (linker N my_cores) Mem.mem 
-    initial_core
-    at_external
-    after_external
-    halted 
-    (fun _ : ge_ty => corestep)
-    corestep_not_at_external    
-    corestep_not_halted 
-    at_external_halted_excl.
-
-(** The linking semantics function \mathcal{L} is deterministic:
-    \mathcal{L}(M1,...,Mn) is deterministic as long as M1, ..., Mn are. *)
-
-Lemma linking_det 
-  (dets : forall ix : 'I_N, 
-    semantics_lemmas.corestep_fun (Modsem.sem (my_cores ix))) :
-  semantics_lemmas.corestep_fun coresem.
-Proof.
-move=> ge m c m' c' m'' c''.
-move/CorestepP=> H1; move/CorestepP=> H2. 
-inversion H2; subst.
-{ inversion H1; subst; first by case: (dets _ _ _ _ _ _ _ _ H H0)=> -> ->.
-  by apply semantics.corestep_not_at_external in H; rewrite H in H0.
-  by apply semantics.corestep_not_halted in H; rewrite H in H4. }
-{ inversion H1; subst.
-  by apply semantics.corestep_not_at_external in H6; rewrite H6 in H.
-  move: H0 H7 H3 H8; rewrite H6 in H; case: H=> <- _ eq0 ->; case=> eq1; subst.
-  move=> ->; case=> eq_ix; subst d_ix0.
-  rewrite H4 in H9; case: H9; move=> ?; subst.
-  rewrite H10 in H5; case: H5=> ->.
-  by split=> //; f_equal; f_equal; apply: proof_irr.
-  case: (semantics.at_external_halted_excl 
-          (Modsem.sem (my_cores (Core.i (peekCore c')))) (Core.c (peekCore c'))).
-  by rewrite H. by rewrite H8. }
-{ inversion H1; subst.
-  by apply semantics.corestep_not_halted in H6; rewrite H6 in H3. 
-  case: (semantics.at_external_halted_excl 
-          (Modsem.sem (my_cores (Core.i (peekCore c')))) (Core.c (peekCore c'))).
-  by rewrite H6. by rewrite H3. 
-  rewrite H8 in H3; case: H3=> eq1; subst. 
-  rewrite H0 in H7; case: H7=> eq2; subst.
-  by rewrite H5 in H10; case: H10=> <-. }
-Qed.
-
-End linkerSem. End LinkerSem.
-
-(** ** Linking Effect Semantics *)
-
-Section effingLinker.
-
-Variable N : pos. 
-Variable my_cores : 'I_N -> Modsem.t. 
-Variable my_fun_tbl : ident -> option 'I_N.
-
-Import Linker.
-
-Definition effstep0 U (l: linker N my_cores) m (l': linker N my_cores) m' := 
-  let: c   := peekCore l in
-  let: ix  := c.(Core.i) in
-  let: sem := (my_cores ix).(Modsem.sem) in
-  let: F   := (my_cores ix).(Modsem.F) in
-  let: V   := (my_cores ix).(Modsem.V) in
-  let: ge  := (my_cores ix).(Modsem.ge) in
-    exists c', 
-      @effstep (Genv.t F V) _ sem ge U (Core.c c) m c' m'
-   /\ l' = updCore l (Core.upd c c').
-
-Lemma effstep0_unchanged U l m l' m' : 
-  effstep0 U l m l' m' ->
-  Mem.unchanged_on (fun b ofs => U b ofs = false) m m'.
-Proof. 
-rewrite/effstep0; case=> ? [STEP].
-by move: {STEP}(effax1 STEP)=> [STEP]UNCH H2.
-Qed.
-
-Lemma effstep0_corestep0 U l m l' m' : 
-  effstep0 U l m l' m' -> LinkerSem.corestep0 l m l' m'.
-Proof. 
-rewrite/effstep0/LinkerSem.corestep0; case=> c' [STEP].
-move: {STEP}(effax1 STEP)=> [STEP]UNCH H2.
-by exists c'; split.
-Qed.
-
-Lemma effstep0_forward U l m l' m' : 
-  effstep0 U l m l' m' -> mem_forward m m'.
-Proof. 
-move/effstep0_corestep0; rewrite/LinkerSem.corestep0. 
-by move=> []c' []STEP H1; apply: {STEP}(corestep_fwd STEP). 
-Qed.
-
-Definition inner_effstep (ge: ge_ty)
-  (l: linker N my_cores) m (l': linker N my_cores) m' := 
-  [/\ LinkerSem.corestep l m l' m' 
-    & LinkerSem.corestep0 l m l' m' -> exists U, effstep0 U l m l' m'].
-
-Definition effstep (ge: ge_ty) V
-  (l: linker N my_cores) m (l': linker N my_cores) m' := 
-  [/\ LinkerSem.corestep l m l' m' 
-    , LinkerSem.corestep0 l m l' m' -> effstep0 V l m l' m'
-    & ~LinkerSem.corestep0 l m l' m' -> forall b ofs, ~~ V b ofs].
-
-Section csem.
-
-Notation mycsem := (LinkerSem.coresem N my_cores my_fun_tbl).
-
-Program Definition csem 
-  : CoreSemantics ge_ty (linker N my_cores) Mem.mem := 
-  Build_CoreSemantics _ _ _
-    (initial_core mycsem)
-    (at_external mycsem)
-    (after_external mycsem)
-    (halted mycsem) 
-    inner_effstep _ _ _.
-
-Next Obligation. 
-move: H; rewrite/inner_effstep=> [[H1] H2]. 
-by apply: (LinkerSem.corestep_not_at_external ge H1).
-Qed.
-
-Next Obligation.
-move: H; rewrite/inner_effstep=> [[H1] H2]. 
-by apply: (LinkerSem.corestep_not_halted ge H1).
-Qed.
-
-Next Obligation. by apply: (LinkerSem.at_external_halted_excl). Qed.
-
-End csem.
-
-Lemma linking_det 
-  (dets : forall ix : 'I_N, 
-    semantics_lemmas.corestep_fun (Modsem.sem (my_cores ix))) :
-  semantics_lemmas.corestep_fun csem.
-Proof.
-move=> m m' m'' ge c c' c''; rewrite /= /inner_effstep => [][]H1 _ []H2 _.
-case: (@LinkerSem.linking_det N my_cores my_fun_tbl dets _ _ _ _ _ _ _ H1 H2).
-by refine ge. 
-by move=> -> ->.
-Qed.
-
-Program Definition coopsem := Build_CoopCoreSem _ _ csem _.
-
-Next Obligation. 
-move: CS; case; move=>[H1|[<- [H0 H1]]]. 
-by move/(_ H1)=>{H1} [U EFF]; apply (effstep0_forward EFF).
-by move=> ?; apply mem_forward_refl.
-Qed.
-
-Program Definition effsem := Build_EffectSem _ _ coopsem effstep _ _ _.
-
-Next Obligation. 
-move: H=>[H1]H2; split. 
-by split=> //; move=> H3; move: {H2 H3}(H2 H3)=> STEP; exists M.
-case: H1=> [H1|[<- [H0 H1]]]=> //. 
-by move: (H2 H1)=> H3; apply: (effstep0_unchanged H3).
-Qed.
-
-Next Obligation.
-move: H; rewrite/inner_effstep=> [[[H1|[<- [H0 H1]]]]] H2=> //.
-move: (H2 H1)=> {H2}[U H3]; exists U; split=> //.
-by left; apply: (effstep0_corestep0 H3).
-by exists [fun _ _ => false]; split=> //; right.
-Qed.
-
-Next Obligation.
-move: H; rewrite/effstep=> [][]; case.
-move=> H; move/(_ H); rewrite/effstep0. 
-by move=> []? []H2 _ _; apply: (effstep_valid _ _ _ _ _ _ _ H2 _ _ H0).
-by move=> []_ []nstep _ _; move/(_ nstep b z); rewrite H0.
-Qed.
-
-End effingLinker.
+Notation ctl := (ctl sem).
+Notation num_threads := (num_threads tp).
+Notation thread_pool := (t sem).
+
+Definition addThread (c : ctl) : thread_pool :=
+  let: new_num_threads := pos_incr num_threads in
+  let: new_tid := ordinal_pos_incr num_threads in
+  @mk sem new_num_threads  (fun (n : 'I_new_num_threads) => 
+      match unlift new_tid n with
+        | None => c
+        | Some n' => tp n'
+      end) 
+   (counter tp).+1.
+
+Definition updThread (tid : 'I_num_threads) (c' : ctl) : thread_pool :=
+  @mk sem num_threads (fun (n : 'I_num_threads) => 
+      if n == tid then c' else tp n) 
+  (counter tp).+1.
+
+Definition getThread (tid : 'I_num_threads) : ctl := tp tid.
+  
+End poolDefs.
+
+Section poolLemmas.
+
+Context {sem : Modsem.t} {next : block} (tp : ThreadPool.t sem).
+
+Import ThreadPool.
+
+Lemma gssThread (tid : 'I_(num_threads tp)) c' : 
+  getThread (updThread tp tid c') tid = c'.
+Proof. by rewrite /getThread /updThread /= eq_refl. Qed.
+
+Lemma gsoThread (tid tid' : 'I_(num_threads tp)) c' :
+  tid' != tid -> getThread (updThread tp tid c') tid' = getThread tp tid'.
+Proof. by rewrite /getThread /updThread /=; case Heq: (tid' == tid). Qed.
+
+Lemma getAddThread c tid :
+  tid = ordinal_pos_incr (num_threads tp) ->
+  getThread (addThread tp c) tid = c.
+Proof. by rewrite /getThread /addThread /= => <-; rewrite unlift_none. Qed.
+
+End poolLemmas.
+
+Module Concur. Section Concur.
+
+Import ThreadPool.
+
+Context {sem : Modsem.t} (tp : ThreadPool.t sem).
+
+Notation thread_pool := (t sem).
+Notation the_ge := (Modsem.ge sem).
+Notation the_sem := (Modsem.sem sem).
+Notation perm_map := PermMap.t.
+
+Variable  aggelos : nat -> perm_map.
+Variable schedule : nat -> nat.
+
+Inductive step : thread_pool -> mem -> thread_pool -> mem -> Prop :=
+  | step_congr : 
+      forall tp m c m' (c' : Modsem.C sem),
+      let: n := counter tp in
+      let: tid0 := schedule n in
+      forall (tid0_lt_pf :  tid0 < num_threads tp),
+      let: tid := Ordinal tid0_lt_pf in
+      getThread tp tid = Krun c ->
+      semantics.corestep the_sem the_ge c m c' m' ->
+      step tp m (updThread tp tid (Krun c')) m'
+
+  | step_lock_into :
+      forall tp m c b ofs,
+      let: n := counter tp in
+      let: tid0 := schedule n in
+      forall (tid0_lt_pf :  tid0 < num_threads tp),
+      let: tid := Ordinal tid0_lt_pf in
+      getThread tp tid = Krun c ->
+      semantics.at_external the_sem c = Some (LOCK, LOCK_SIG, Vptr b (Int.repr ofs)::nil) ->
+      step tp m (updThread tp tid (Klock b ofs c)) m
+
+  | step_lock_exec :
+      forall tp m c m'' c' m' b ofs,
+      let: n := counter tp in
+      let: tid0 := schedule n in
+      forall (tid0_lt_pf :  tid0 < num_threads tp),
+      let: tid := Ordinal tid0_lt_pf in
+      getThread tp tid = Klock b ofs c ->
+      semantics.at_external the_sem c = Some (LOCK, LOCK_SIG, Vptr b (Int.repr ofs)::nil) ->
+      Mem.load Mint32 m b ofs = Some (Vint Int.one) ->
+      Mem.store Mint32 m b ofs (Vint Int.zero) = Some m'' ->
+      semantics.after_external the_sem (Some (Vint Int.zero)) c = Some c' ->
+      updPermMap m'' (aggelos n) = Some m' -> 
+      step tp m (updThread tp tid (Krun c')) m'
+
+  | step_unlock :
+      forall tp m c m'' c' m' b ofs,
+      let: n := counter tp in
+      let: tid0 := schedule n in
+      forall (tid0_lt_pf :  tid0 < num_threads tp),
+      let: tid := Ordinal tid0_lt_pf in
+      getThread tp tid = Krun c ->
+      semantics.at_external the_sem c = Some (UNLOCK, UNLOCK_SIG, Vptr b (Int.repr ofs)::nil) ->
+      Mem.load Mint32 m b ofs = Some (Vint Int.zero) ->
+      Mem.store Mint32 m b ofs (Vint Int.one) = Some m'' ->
+      semantics.after_external the_sem (Some (Vint Int.zero)) c = Some c' ->
+      updPermMap m'' (aggelos n) = Some m' -> 
+      step tp m (updThread tp tid (Krun c')) m'.
+
+End Concur. End Concur.
